refacta

fizzBuzz.fst
@@ -12,13 +12,13 @@ module U = FStar.UInt
 module U32 = FStar.UInt32
 module ST = FStar.HyperStack.ST
 
-val normal_loop: src:B.buffer U32.t -> len:U32.t -> Stack string
-  (requires fun h0 -> B.live h0 src /\ B.length src = U32.v len )
+val fizz_buzz: len:U32.t -> Stack C.exit_code
+  (requires fun _ -> true)
   (ensures fun _ _ _ -> true)
-let normal_loop src len =
-  let inv h (i: nat) = B.live h src in
+let fizz_buzz len =
+  let inv h (i: nat) = bool in
   let body (i: U32.t{ 0 <= U32.v i /\ U32.v i < U32.v len }): Stack unit
-    (requires (fun h -> inv h (U32.v i)))
+    (requires (fun _ -> true))
     (ensures (fun _ _ _ -> true))
   =
     let count: U32.t = U32.(i +^ 1ul) in
@@ -30,16 +30,9 @@ let normal_loop src len =
     else printf "%ul: \n" count done
   in
   C.Loops.for 0ul len inv body;
-  (* return *) "LOOP DONE!\n"
+  (* return *) C.EXIT_SUCCESSl
 
 let main ()
 =
-  push_frame ();
-  // let src = B.alloca_of_list a in
-  // let len: U32.t = U32.uint_to_t (FStar.List.Tot.length a)  in
-  let listSize = 10000ul in
-  let fillData = 0ul in
-  let src = B.alloca fillData listSize in
-  let _ = normal_loop src listSize in
-  pop_frame ();
+  let _ = fizz_buzz 30ul in
   C.EXIT_SUCCESS
